assembler/Symbtablegenproof1.v
@@ -32,6 +32,8 @@ Hypothesis TRANSF: match_prog instr_size prog tprog.
 
 Let match_states := match_states instr_size prog tprog.
 Let init_mem_pres_inject := init_mem_pres_inject instr_size instr_size_bound prog tprog TRANSF.
+Let initial_state_gen_pres_match := initial_state_gen_pres_match instr_size instr_size_bound prog tprog TRANSF.
+  
 (* set hypothesis *)
 Lemma transf_initial_states : forall rs st1,
     RealAsm.initial_state prog st1 ->
@@ -44,189 +46,14 @@ Proof.
   inv INIT.
   exploit (init_mem_pres_inject m0);eauto.
   intros (m0' & INITM' & MINJ).
-  (* exploit (Mem.alloc_parallel_inject (Mem.flat_inj (Mem.support m0)) *)
-  (*              m0 m0' 0 (max_stacksize + align (size_chunk Mptr) 8) *)
-  (*              m1 stk 0 (max_stacksize + align (size_chunk Mptr) 8));eauto;try lia. *)
-  (*** TODO  *)
-  exploit (Mem.valid_new_block m0);eauto. unfold Mem.valid_block. intros VALIDSTK.
-  caseEq (Mem.alloc m0' 0 (max_stacksize + align (size_chunk Mptr) 8)).
-  intros m1'  stk'  H0'.
-  exploit (alloc_stack_pres_inject m0 m0');eauto.
-  intros (MINJ1 &  STK &  MATINJ1). subst.  
-  exploit (storev_pres_match_inj Mptr m1 m2);eauto.
-  intros MATINJ2.
-  edestruct storev_pres_inject as (m2' & ST & SMINJ). apply H1. apply MINJ1. econstructor. econstructor.
-  (* stk' is valid *)
-  unfold Mem.flat_inj. destruct (Mem.sup_dec stk' (Mem.support m1)).
-  eauto. congruence.
-  eapply eq_refl. constructor.
-  (* regset *)
-  set (rs0' := rs # PC <- (Genv.symbol_address tge tprog.(prog_main) Ptrofs.zero)
-           # RA <- Vnullptr
-           # RSP <- (Vptr stk' (Ptrofs.sub (Ptrofs.repr (max_stacksize + align (size_chunk Mptr) 8)) (Ptrofs.repr (size_chunk Mptr))))) in *.
 
-  (* instantiate the initial state*)
-  exists (State rs0' m2').
-  split. 
-  (* initial_state *)
-  - econstructor;eauto.
-    econstructor;eauto.
-  - econstructor;eauto.
-    unfold regset_inject. intros.
-    
-    unfold rs0',rs0.
-    apply val_inject_set.
-    apply val_inject_set.
-    apply val_inject_set.
-    auto.
-      (* main function *)
-      destr_in TRANSF'. simpl.
-     exploit (agree_inj_globs (Mem.flat_inj (Mem.support m2)) MATINJ2 ((AST.prog_main prog)) bmain). auto.
-     intros (bmain' & ofs' & MAIN' & MAININJ).
-     (* proof bmain is valid in m2 support *)
-     exploit (Genv.find_symbol_not_fresh). apply H. apply H2. intros VALIDMAIN0.
-     exploit (Mem.valid_block_alloc). apply H0. apply VALIDMAIN0. intros VALIDMAIN1.
-     exploit (Mem.support_store). apply H1. intros SUPEQ.
-     unfold Mem.valid_block in VALIDMAIN1.
-     rewrite <- SUPEQ in VALIDMAIN1. unfold Mem.flat_inj in MAININJ.
-     destruct (Mem.sup_dec bmain (Mem.support m2));try congruence.
-     destr_in MAININJ.
-     unfold Genv.symbol_address.
-     rewrite MAIN'. econstructor.
-     unfold Mem.flat_inj. destruct (Mem.sup_dec bmain' (Mem.support m2));try congruence. eauto.
-     rewrite Ptrofs.add_unsigned. rewrite Ptrofs.add_zero.
-     rewrite <- H6. rewrite Z.add_0_r. rewrite Ptrofs.unsigned_zero. auto.
-     constructor.
-     cbn [Val.offset_ptr].
-     rewrite Ptrofs.sub_add_opp.
-     econstructor.
-     (* prove SSAsm.stkblock = stk' = stk *)
-     exploit (Genv.init_mem_stack). eapply H. intros.
-     exploit (init_mem_stack). eapply INITM'. intros.
-     assert (stk' = SSAsm.stkblock).
-     exploit Mem.alloc_result. eapply H0.
-     unfold Mem.nextblock. unfold Mem.fresh_block. rewrite H3.
-     simpl. intros. rewrite H5. unfold SSAsm.stkblock. auto.
-     (* prove stk' in support m2 *)
-     rewrite <- H5.
-     exploit Mem.support_storev. apply H1. intros.
-     rewrite <- H6. unfold Mem.flat_inj.
-     destruct Mem.sup_dec. eauto.
-     congruence.
-     rewrite Ptrofs.add_zero. auto.
-     (* glob block valid *)
-     
-     unfold glob_block_valid. intros.
-     exploit (Genv.find_def_not_fresh). apply H. apply H3.
-     unfold Mem.valid_block. intros.
-     exploit Mem.support_alloc. apply H0. 
-     exploit Mem.support_storev. apply H1.
-     intros. rewrite <- H5. rewrite H6.
-     exploit Mem.sup_include_incr. apply H4. auto.
+  (* initial state gen preserves injection *)
+  exploit (initial_state_gen_pres_match m0 m0' m' rs0 rs);eauto.
+  intros (st & INITGEN & MATCH).
+  exists st. econstructor. econstructor;eauto.
+  unfold match_states. auto.
 Qed.
 
-
-Theorem step_simulation:
-  forall S1 t S2,
-    RealAsm.step instr_size ge S1 t S2 ->
-    forall S1' (MS: match_states S1 S1'),
-    exists S2',
-      step instr_size tge S1' t S2' /\
-      match_states S2 S2'.
-Proof.
-  destruct 1; intros; inv MS.
-
-  - (* Internal step *)
-    unfold regset_inject in RSINJ. generalize (RSINJ Asm.PC). rewrite H. 
-    inversion 1; subst.
-    exploit (agree_inj_instrs (Mem.flat_inj (Mem.support m)) MATCHINJ b b2 f ofs delta i); eauto.
-    intros FIND.
-    exploit (exec_instr_step (Mem.flat_inj (Mem.support m)) rs rs'0 m m'0 rs' m' i); eauto.
-    intros (rs2' & m2' & FEXEC & MS1).
-    exists (State rs2' m2'). split; auto.
-    eapply exec_step_internal; eauto.
-    eapply (agree_inj_int_funct (Mem.flat_inj (Mem.support m)) MATCHINJ); eauto.
-        
-  - (* Builtin *)
-    unfold regset_inject in RSINJ. generalize (RSINJ Asm.PC). rewrite H.
-    inversion 1; subst.
-    exploit (agree_inj_instrs (Mem.flat_inj (Mem.support m)) MATCHINJ b b2 f ofs delta (Asm.Pbuiltin ef args res)); auto.
-    intros FIND.
-    exploit (eval_builtin_args_inject (Mem.flat_inj (Mem.support m)) m m'0 rs rs'0 (rs Asm.RSP) (rs'0 Asm.RSP) args vargs); auto.
-    intros (vargs' & EBARGS & ARGSINJ).
-    assert (Globalenvs.Genv.to_senv ge = (Genv.genv_senv tge)) as SENVEQ. 
-    { eapply transf_prog_pres_senv; eauto. }
-    exploit (external_call_inject ge (Mem.flat_inj (Mem.support m)) vargs vargs' m m'0 m' vres t ef);eauto.
-    rewrite SENVEQ.
-    intros (j' & vres2 & m2' & EXTCALL & RESINJ & MINJ' & INJINCR & INJSEP & INJ).
-    set (rs' := nextinstr_nf (Ptrofs.repr (instr_size (Pbuiltin ef args res)))
-                             (set_res res vres2 (undef_regs (map preg_of (Machregs.destroyed_by_builtin ef)) rs'0))).
-    exploit (fun b ofs => exec_step_builtin instr_size tge b ofs
-                                         ef args res rs'0  m'0 vargs' t vres2 rs' m2'); eauto. 
-    eapply (agree_inj_int_funct (Mem.flat_inj (Mem.support m)) MATCHINJ); eauto.
-    intros FSTEP. eexists; split; eauto.
-    eapply match_states_intro with (j:=j'); eauto.
-    (* Supposely the following propreties can proved by separation property of injections *)
-    + eapply (inject_pres_match_sminj (Mem.flat_inj (Mem.support m))); eauto.
-    + subst rs'. intros. 
-      assert (regset_inject j' rs rs'0) by 
-          (eapply regset_inject_incr; eauto).
-      set (dregs := (map Asm.preg_of (Machregs.destroyed_by_builtin ef))) in *.
-      generalize (undef_regs_pres_inject j' rs rs'0 dregs H5). intros.
-      set (rs1 := (Asm.undef_regs dregs rs)) in *.
-      set (rs2 := (Asm.undef_regs dregs rs'0)) in *.
-      generalize (fun h => set_res_pres_inject res j' 
-                  rs1 rs2 h vres vres2 RESINJ).
-      set (rs3 := (Asm.set_res res vres rs1)) in *.
-      set (rs4 := (Asm.set_res res vres2 rs2)) in *.
-      intros.
-      eapply nextinstr_nf_pres_inject. auto.
-      (* eauto with inject_db. *)
-    + eapply extcall_pres_glob_block_valid; eauto.
-
-  - (* External call *)
-    unfold regset_inject in RSINJ. generalize (RSINJ Asm.PC). rewrite H. 
-    inversion 1; subst. rewrite Ptrofs.add_zero_l in H6.
-    exploit loadv_inject. apply MINJ. apply LOADRA. eauto. intros (v2 & LRA & VI).
-    edestruct (extcall_arguments_inject) as (args2 & ARGSINJ & EXTCALLARGS); eauto.
-    apply regset_inject_expand. eauto.
-    apply Val.offset_ptr_inject. eauto.
-    assert (Globalenvs.Genv.to_senv ge = (Genv.genv_senv tge)) as SENVEQ. 
-    { eapply transf_prog_pres_senv; eauto. }
-    exploit (external_call_inject ge (Mem.flat_inj (Mem.support m)) args args2 ); eauto.
-    rewrite SENVEQ.
-    
-    intros (j' & res' & m2'' & EXTCALL & RESINJ & MINJ' & INJINCR & INJSEP & INJ).
-    exploit (fun ofs => exec_step_external instr_size tge b2 ofs ef args2 res'); eauto.
-    eapply agree_inj_ext_funct; eauto.
-    + intro; subst. inv VI. congruence.
-    + intros FSTEP. eexists. split. apply FSTEP.
-      eapply match_states_intro with (j := j'); eauto.
-      * eapply (inject_pres_match_sminj (Mem.flat_inj (Mem.support m))); eauto.
-      * assert (regset_inject j' rs rs'0) by 
-            (eapply regset_inject_incr; eauto).
-        (* set (dregs := (map Asm.preg_of Conventions1.destroyed_at_call)) in *. *)
-        (* generalize (undef_regs_pres_inject j' rs rs'0 dregs H4). intros. *)
-        (* set (rs1 := (Asm.undef_regs dregs rs)) in *. *)
-        (* set (rs2 := (Asm.undef_regs dregs rs'0)) in *. *)
-        (* set (cdregs := (CR Asm.ZF :: CR Asm.CF :: CR Asm.PF :: CR Asm.SF :: CR Asm.OF :: nil)) in *. *)
-        (* generalize (undef_regs_pres_inject j' rs1 rs2 cdregs). intros. *)
-        (* set (rs3 := (Asm.undef_regs cdregs rs1)) in *. *)
-        (* set (rs4 := (Asm.undef_regs cdregs rs2)) in *. *)
-        (* generalize (set_pair_pres_inject j' rs3 rs4 res res'  *)
-        (*                                  (Asm.loc_external_result (ef_sig ef))). *)
-        intros.
-        apply regset_inject_expand; auto.
-        apply regset_inject_expand; auto.
-        apply regset_inject_expand; auto.
-        eapply set_pair_pres_inject.
-        unfold regset_inject.
-        eapply val_inject_undef_caller_save_regs.
-        auto. auto.
-        eapply val_inject_incr; eauto.
-        apply Val.offset_ptr_inject; eauto.
-      * eapply extcall_pres_glob_block_valid; eauto.
-Qed.
 
 
 (** ** Matching of the Final States*)
@@ -250,6 +77,7 @@ Proof.
   intros. apply forward_simulation_step with match_states.
   - simpl. intros. 
     unfold match_prog in TRANSF. unfold transf_program in TRANSF.
+    clear init_mem_pres_inject initial_state_gen_pres_match.
     repeat destr_in TRANSF. cbn.
     auto.
     (* rewrite add_external_globals_pres_senv. cbn. auto. *)
@@ -264,6 +92,8 @@ Qed.
 
 End PRESERVATION.
 
-Instance symbtablegen_transflink (instr_size: instruction -> Z):
+Instance symbtablegen_transflink:
   TransfLink (match_prog instr_size).
 Admitted.
+
+End WITH_INSTR_SIZE.
