x86/SymbtablegenproofArchi.v
@@ -752,15 +752,24 @@ Proof.
   eauto.
 Qed.
 
+Lemma prog_main_eq: AST.prog_main prog = prog_main tprog.
+Proof.
+  unfold match_prog,transf_program in *.
+  repeat destr_in TRANSF.
+  simpl. auto.
+Qed.
+
 Let alloc_stack_pres_inject := alloc_stack_pres_inject instr_size instr_size_bound prog tprog TRANSF.
 Let storev_pres_match_inj := storev_pres_match_inj instr_size prog tprog.
+Let agree_inj_globs := agree_inj_globs instr_size prog tprog.
 
-Lemma initial_state_gen_pres_inject: forall m0 m0' m1 rs0 rs
+
+Lemma initial_state_gen_pres_match: forall m0 m0' m1 rs0 rs
     (INIT: Genv.init_mem prog = Some m0)
     (INIT': init_mem instr_size tprog = Some m0'),
     magree (Mem.flat_inj (Mem.support m0)) m0 m0' ->
     RealAsmArchi.initial_stack_regset prog m0 m1 rs0 ->
-    exists st, initial_state_gen instr_size tprog rs m0' st.
+    exists st, initial_state_gen instr_size tprog rs m0' st /\ match_states (State rs0 m1) st.
 Proof.
   intros. inv H0.
   exploit (Mem.valid_new_block m0);eauto. unfold Mem.valid_block. intros VALIDSTK.
@@ -782,8 +791,178 @@ Proof.
 
   (* instantiate the initial state*)
   exists (State rs0' m2').
+  split.
   econstructor;eauto.
+
+  econstructor;eauto.
+  unfold regset_inject. intros.
+    
+  unfold rs0',rs1.
+  apply val_inject_set.
+  apply val_inject_set.
+  apply val_inject_set.
+  auto.
+  (* main function *)
+  generalize TRANSF. intros TRANSF'.
+  exploit (agree_inj_globs (Mem.flat_inj (Mem.support m1)) MATINJ2 ((AST.prog_main prog)) bmain). auto.
+  intros (bmain' & ofs' & MAIN' & MAININJ).
+  (* proof bmain is valid in m2 support *)
+  exploit (Genv.find_symbol_not_fresh). apply INIT. apply H3. intros VALIDMAIN0.
+  exploit (Mem.valid_block_alloc). apply H1. apply VALIDMAIN0. intros VALIDMAIN1.
+  exploit (Mem.support_store). apply H2. intros SUPEQ.
+  unfold Mem.valid_block in VALIDMAIN1.
+  rewrite <- SUPEQ in VALIDMAIN1. unfold Mem.flat_inj in MAININJ.
+  destruct (Mem.sup_dec bmain (Mem.support m1));try congruence.
+  destr_in MAININJ.
+  unfold Genv.symbol_address.
+  unfold tge.
+  erewrite <- prog_main_eq.  
+  rewrite MAIN'. econstructor.
+  unfold Mem.flat_inj. destruct (Mem.sup_dec bmain' (Mem.support m1));try congruence. eauto.
+  rewrite Ptrofs.add_unsigned. rewrite Ptrofs.add_zero.
+  rewrite <- H5. rewrite Z.add_0_r. rewrite Ptrofs.unsigned_zero. auto.
+
+  constructor.
+  cbn [Val.offset_ptr].
+  rewrite Ptrofs.sub_add_opp.
+  econstructor.
+
+  (* prove SSAsm.stkblock = stk' = stk *)
+  exploit (Genv.init_mem_stack). eapply INIT. intros.
+  exploit (init_mem_stack). eapply INIT'. intros.
+  assert (stk' = RealAsmArchi.stkblock).
+  exploit Mem.alloc_result. eapply H1.
+  unfold Mem.nextblock. unfold Mem.fresh_block. rewrite H0.
+  simpl. intros. rewrite H5. unfold RealAsmArchi.stkblock. auto.
+
+  (* prove stk' in support m2 *)
+  rewrite <- H5.
+  exploit Mem.support_storev. apply H2. intros.
+  rewrite <- H6. unfold Mem.flat_inj.
+  destruct Mem.sup_dec. eauto.
+  congruence.
+  rewrite Ptrofs.add_zero. auto.
+  (* glob block valid *)
+  
+  unfold glob_block_valid. intros.
+  unfold Symbtablegenproof.glob_block_valid. intros.
+  exploit (Genv.find_def_not_fresh). apply INIT. apply H0.
+  unfold Mem.valid_block. intros.
+  exploit Mem.support_alloc. apply H1. 
+  exploit Mem.support_storev. apply H2.
+  intros. rewrite <- H5. rewrite H6.
+  exploit Mem.sup_include_incr. apply H4. auto.
+
 Qed.
+
+
+Let agree_inj_instrs := agree_inj_instrs instr_size prog tprog.
+Let agree_inj_int_funct := agree_inj_int_funct instr_size prog tprog.
+Let inject_pres_match_sminj := inject_pres_match_sminj instr_size prog tprog.
+
+Theorem step_simulation:
+  forall S1 t S2,
+    RealAsmArchi.step instr_size ge S1 t S2 ->
+    forall S1' (MS: match_states S1 S1'),
+    exists S2',
+      step instr_size tge S1' t S2' /\
+      match_states S2 S2'.
+Proof.
+  destruct 1; intros; inv MS.
+
+  - (* Internal step *)
+    unfold regset_inject in RSINJ. generalize (RSINJ Asm.PC). rewrite H. 
+    inversion 1; subst.
+    exploit (agree_inj_instrs (Mem.flat_inj (Mem.support m)) MATCHINJ b b2 f ofs delta i); eauto.
+    intros FIND.
+    exploit (exec_instr_step (Mem.flat_inj (Mem.support m)) rs rs'0 m m'0 rs' m' i); eauto.
+    intros (rs2' & m2' & FEXEC & MS1).
+    exists (State rs2' m2'). split; auto.
+    eapply exec_step_internal; eauto.
+    (* eapply (agree_inj_int_funct (Mem.flat_inj (Mem.support m)) MATCHINJ); eauto. *)
+        
+  (* - (* Builtin *) *)
+  (*   unfold regset_inject in RSINJ. generalize (RSINJ Asm.PC). rewrite H. *)
+  (*   inversion 1; subst. *)
+  (*   exploit (agree_inj_instrs (Mem.flat_inj (Mem.support m)) MATCHINJ b b2 f ofs delta (Asm.Pbuiltin ef args res)); auto. *)
+  (*   intros FIND. *)
+  (*   exploit (eval_builtin_args_inject (Mem.flat_inj (Mem.support m)) m m'0 rs rs'0 (rs Asm.RSP) (rs'0 Asm.RSP) args vargs); auto. *)
+  (*   intros (vargs' & EBARGS & ARGSINJ). *)
+  (*   assert (Globalenvs.Genv.to_senv ge = (Genv.genv_senv tge)) as SENVEQ.  *)
+  (*   { eapply transf_prog_pres_senv; eauto. } *)
+  (*   exploit (external_call_inject ge (Mem.flat_inj (Mem.support m)) vargs vargs' m m'0 m' vres t ef);eauto. *)
+  (*   rewrite SENVEQ. *)
+  (*   intros (j' & vres2 & m2' & EXTCALL & RESINJ & MINJ' & INJINCR & INJSEP & INJ). *)
+  (*   set (rs' := nextinstr_nf (Ptrofs.repr (instr_size (Pbuiltin ef args res))) *)
+  (*                            (set_res res vres2 (undef_regs (map preg_of (Machregs.destroyed_by_builtin ef)) rs'0))). *)
+  (*   exploit (fun b ofs => exec_step_builtin instr_size tge b ofs *)
+  (*                                        ef args res rs'0  m'0 vargs' t vres2 rs' m2'); eauto.  *)
+  (*   eapply (agree_inj_int_funct (Mem.flat_inj (Mem.support m)) MATCHINJ); eauto. *)
+  (*   intros FSTEP. eexists; split; eauto. *)
+  (*   eapply match_states_intro with (j:=j'); eauto. *)
+  (*   (* Supposely the following propreties can proved by separation property of injections *) *)
+  (*   + eapply (inject_pres_match_sminj (Mem.flat_inj (Mem.support m))); eauto. *)
+  (*   + subst rs'. intros.  *)
+  (*     assert (regset_inject j' rs rs'0) by  *)
+  (*         (eapply regset_inject_incr; eauto). *)
+  (*     set (dregs := (map Asm.preg_of (Machregs.destroyed_by_builtin ef))) in *. *)
+  (*     generalize (undef_regs_pres_inject j' rs rs'0 dregs H5). intros. *)
+  (*     set (rs1 := (Asm.undef_regs dregs rs)) in *. *)
+  (*     set (rs2 := (Asm.undef_regs dregs rs'0)) in *. *)
+  (*     generalize (fun h => set_res_pres_inject res j'  *)
+  (*                 rs1 rs2 h vres vres2 RESINJ). *)
+  (*     set (rs3 := (Asm.set_res res vres rs1)) in *. *)
+  (*     set (rs4 := (Asm.set_res res vres2 rs2)) in *. *)
+  (*     intros. *)
+  (*     eapply nextinstr_nf_pres_inject. auto. *)
+  (*     (* eauto with inject_db. *) *)
+  (*   + eapply extcall_pres_glob_block_valid; eauto. *)
+
+  - (* External call *)
+    unfold regset_inject in RSINJ. generalize (RSINJ Asm.PC). rewrite H. 
+    inversion 1; subst. rewrite Ptrofs.add_zero_l in H6.
+    exploit loadv_inject. apply MINJ. apply LOADRA. eauto. intros (v2 & LRA & VI).
+    edestruct (extcall_arguments_inject) as (args2 & ARGSINJ & EXTCALLARGS); eauto.
+    apply regset_inject_expand. eauto.
+    apply Val.offset_ptr_inject. eauto.
+    assert (Globalenvs.Genv.to_senv ge = (Genv.genv_senv tge)) as SENVEQ. 
+    { eapply transf_prog_pres_senv; eauto. }
+    exploit (external_call_inject ge (Mem.flat_inj (Mem.support m)) args args2 ); eauto.
+    rewrite SENVEQ.
+    
+    intros (j' & res' & m2'' & EXTCALL & RESINJ & MINJ' & INJINCR & INJSEP & INJ).
+    exploit (fun ofs => exec_step_external instr_size tge b2 ofs ef args2 res'); eauto.
+    eapply agree_inj_ext_funct; eauto.
+    + intro; subst. inv VI. congruence.
+    + intros FSTEP. eexists. split. apply FSTEP.
+      eapply match_states_intro with (j := j'); eauto.
+      (* * eapply (inject_pres_match_sminj (Mem.flat_inj (Mem.support m))); eauto. *)
+      * assert (regset_inject j' rs rs'0) by 
+            (eapply regset_inject_incr; eauto).
+        (* set (dregs := (map Asm.preg_of Conventions1.destroyed_at_call)) in *. *)
+        (* generalize (undef_regs_pres_inject j' rs rs'0 dregs H4). intros. *)
+        (* set (rs1 := (Asm.undef_regs dregs rs)) in *. *)
+        (* set (rs2 := (Asm.undef_regs dregs rs'0)) in *. *)
+        (* set (cdregs := (CR Asm.ZF :: CR Asm.CF :: CR Asm.PF :: CR Asm.SF :: CR Asm.OF :: nil)) in *. *)
+        (* generalize (undef_regs_pres_inject j' rs1 rs2 cdregs). intros. *)
+        (* set (rs3 := (Asm.undef_regs cdregs rs1)) in *. *)
+        (* set (rs4 := (Asm.undef_regs cdregs rs2)) in *. *)
+        (* generalize (set_pair_pres_inject j' rs3 rs4 res res'  *)
+        (*                                  (Asm.loc_external_result (ef_sig ef))). *)
+        intros.
+        apply regset_inject_expand; auto.
+        apply regset_inject_expand; auto.
+        apply regset_inject_expand; auto.
+        eapply set_pair_pres_inject.
+        unfold regset_inject.
+        eapply val_inject_undef_caller_save_regs.
+        auto. auto.
+        eapply val_inject_incr; eauto.
+        apply Val.offset_ptr_inject; eauto.
+      * eapply extcall_pres_glob_block_valid; eauto.
+Qed.
+
+
 
 End PRESERVATION.
 
